Changed 1 to 1' (= Suc 0)

src/HOL/Auth/NS_Shared.thy
@@ -16,60 +16,60 @@ consts  ns_shared   :: "event list set"
 inductive "ns_shared"
  intros
 	(*Initial trace is empty*)
-  Nil:  "[] \<in> ns_shared"
+  Nil:  "[] \\<in> ns_shared"
 	(*The spy MAY say anything he CAN say.  We do not expect him to
 	  invent new nonces here, but he can also use NS1.  Common to
 	  all similar protocols.*)
-  Fake: "\<lbrakk>evsf \<in> ns_shared;  X \<in> synth (analz (spies evsf))\<rbrakk>
-	 \<Longrightarrow> Says Spy B X # evsf \<in> ns_shared"
+  Fake: "\\<lbrakk>evsf \\<in> ns_shared;  X \\<in> synth (analz (spies evsf))\\<rbrakk>
+	 \\<Longrightarrow> Says Spy B X # evsf \\<in> ns_shared"
 
 	(*Alice initiates a protocol run, requesting to talk to any B*)
-  NS1:  "\<lbrakk>evs1 \<in> ns_shared;  Nonce NA \<notin> used evs1\<rbrakk>
-	 \<Longrightarrow> Says A Server \<lbrace>Agent A, Agent B, Nonce NA\<rbrace> # evs1  \<in>  ns_shared"
+  NS1:  "\\<lbrakk>evs1 \\<in> ns_shared;  Nonce NA \\<notin> used evs1\\<rbrakk>
+	 \\<Longrightarrow> Says A Server \\<lbrace>Agent A, Agent B, Nonce NA\\<rbrace> # evs1  \\<in>  ns_shared"
 
 	(*Server's response to Alice's message.
 	  !! It may respond more than once to A's request !!
 	  Server doesn't know who the true sender is, hence the A' in
 	      the sender field.*)
-  NS2:  "\<lbrakk>evs2 \<in> ns_shared;  Key KAB \<notin> used evs2;
-	  Says A' Server \<lbrace>Agent A, Agent B, Nonce NA\<rbrace> \<in> set evs2\<rbrakk>
-	 \<Longrightarrow> Says Server A
+  NS2:  "\\<lbrakk>evs2 \\<in> ns_shared;  Key KAB \\<notin> used evs2;
+	  Says A' Server \\<lbrace>Agent A, Agent B, Nonce NA\\<rbrace> \\<in> set evs2\\<rbrakk>
+	 \\<Longrightarrow> Says Server A
 	       (Crypt (shrK A)
-		  \<lbrace>Nonce NA, Agent B, Key KAB,
-		    (Crypt (shrK B) \<lbrace>Key KAB, Agent A\<rbrace>)\<rbrace>)
-	       # evs2 \<in> ns_shared"
+		  \\<lbrace>Nonce NA, Agent B, Key KAB,
+		    (Crypt (shrK B) \\<lbrace>Key KAB, Agent A\\<rbrace>)\\<rbrace>)
+	       # evs2 \\<in> ns_shared"
 
 	 (*We can't assume S=Server.  Agent A "remembers" her nonce.
-	   Need A \<noteq> Server because we allow messages to self.*)
-  NS3:  "\<lbrakk>evs3 \<in> ns_shared;  A \<noteq> Server;
-	  Says S A (Crypt (shrK A) \<lbrace>Nonce NA, Agent B, Key K, X\<rbrace>) \<in> set evs3;
-	  Says A Server \<lbrace>Agent A, Agent B, Nonce NA\<rbrace> \<in> set evs3\<rbrakk>
-	 \<Longrightarrow> Says A B X # evs3 \<in> ns_shared"
+	   Need A \\<noteq> Server because we allow messages to self.*)
+  NS3:  "\\<lbrakk>evs3 \\<in> ns_shared;  A \\<noteq> Server;
+	  Says S A (Crypt (shrK A) \\<lbrace>Nonce NA, Agent B, Key K, X\\<rbrace>) \\<in> set evs3;
+	  Says A Server \\<lbrace>Agent A, Agent B, Nonce NA\\<rbrace> \\<in> set evs3\\<rbrakk>
+	 \\<Longrightarrow> Says A B X # evs3 \\<in> ns_shared"
 
 	(*Bob's nonce exchange.  He does not know who the message came
 	  from, but responds to A because she is mentioned inside.*)
-  NS4:  "\<lbrakk>evs4 \<in> ns_shared;  Nonce NB \<notin> used evs4;
-	  Says A' B (Crypt (shrK B) \<lbrace>Key K, Agent A\<rbrace>) \<in> set evs4\<rbrakk>
-	 \<Longrightarrow> Says B A (Crypt K (Nonce NB)) # evs4 \<in> ns_shared"
+  NS4:  "\\<lbrakk>evs4 \\<in> ns_shared;  Nonce NB \\<notin> used evs4;
+	  Says A' B (Crypt (shrK B) \\<lbrace>Key K, Agent A\\<rbrace>) \\<in> set evs4\\<rbrakk>
+	 \\<Longrightarrow> Says B A (Crypt K (Nonce NB)) # evs4 \\<in> ns_shared"
 
 	(*Alice responds with Nonce NB if she has seen the key before.
 	  Maybe should somehow check Nonce NA again.
 	  We do NOT send NB-1 or similar as the Spy cannot spoof such things.
-	  Letting the Spy add or subtract 1 lets him send \<forall>nonces.
+	  Letting the Spy add or subtract 1 lets him send all nonces.
 	  Instead we distinguish the messages by sending the nonce twice.*)
-  NS5:  "\<lbrakk>evs5 \<in> ns_shared;
-	  Says B' A (Crypt K (Nonce NB)) \<in> set evs5;
-	  Says S  A (Crypt (shrK A) \<lbrace>Nonce NA, Agent B, Key K, X\<rbrace>)
-	    \<in> set evs5\<rbrakk>
-	 \<Longrightarrow> Says A B (Crypt K \<lbrace>Nonce NB, Nonce NB\<rbrace>) # evs5 \<in> ns_shared"
+  NS5:  "\\<lbrakk>evs5 \\<in> ns_shared;
+	  Says B' A (Crypt K (Nonce NB)) \\<in> set evs5;
+	  Says S  A (Crypt (shrK A) \\<lbrace>Nonce NA, Agent B, Key K, X\\<rbrace>)
+	    \\<in> set evs5\\<rbrakk>
+	 \\<Longrightarrow> Says A B (Crypt K \\<lbrace>Nonce NB, Nonce NB\\<rbrace>) # evs5 \\<in> ns_shared"
 
 	(*This message models possible leaks of session keys.
 	  The two Nonces identify the protocol run: the rule insists upon
 	  the true senders in order to make them accurate.*)
-  Oops: "\<lbrakk>evso \<in> ns_shared;  Says B A (Crypt K (Nonce NB)) \<in> set evso;
-	  Says Server A (Crypt (shrK A) \<lbrace>Nonce NA, Agent B, Key K, X\<rbrace>)
-	      \<in> set evso\<rbrakk>
-	 \<Longrightarrow> Notes Spy \<lbrace>Nonce NA, Nonce NB, Key K\<rbrace> # evso \<in> ns_shared"
+  Oops: "\\<lbrakk>evso \\<in> ns_shared;  Says B A (Crypt K (Nonce NB)) \\<in> set evso;
+	  Says Server A (Crypt (shrK A) \\<lbrace>Nonce NA, Agent B, Key K, X\\<rbrace>)
+	      \\<in> set evso\\<rbrakk>
+	 \\<Longrightarrow> Notes Spy \\<lbrace>Nonce NA, Nonce NB, Key K\\<rbrace> # evso \\<in> ns_shared"
 
 
 declare Says_imp_knows_Spy [THEN parts.Inj, dest]
@@ -80,8 +80,8 @@ declare image_eq_UN [simp]  (*accelerates proofs involving nested images*)
 
 
 (*A "possibility property": there are traces that reach the end*)
-lemma "A \<noteq> Server \<Longrightarrow> \<exists>N K. \<exists>evs \<in> ns_shared.
-                              Says A B (Crypt K \<lbrace>Nonce N, Nonce N\<rbrace>) \<in> set evs"
+lemma "A \\<noteq> Server \\<Longrightarrow> \\<exists>N K. \\<exists>evs \\<in> ns_shared.
+                              Says A B (Crypt K \\<lbrace>Nonce N, Nonce N\\<rbrace>) \\<in> set evs"
 apply (intro exI bexI)
 apply (rule_tac [2] ns_shared.Nil
        [THEN ns_shared.NS1, THEN ns_shared.NS2, THEN ns_shared.NS3,
@@ -90,8 +90,8 @@ apply possibility
 done
 
 (*This version is similar, while instantiating ?K and ?N to epsilon-terms
-lemma "A \<noteq> Server \<Longrightarrow> \<exists>evs \<in> ns_shared.
-                Says A B (Crypt ?K \<lbrace>Nonce ?N, Nonce ?N\<rbrace>) \<in> set evs"
+lemma "A \\<noteq> Server \\<Longrightarrow> \\<exists>evs \\<in> ns_shared.
+                Says A B (Crypt ?K \\<lbrace>Nonce ?N, Nonce ?N\\<rbrace>) \\<in> set evs"
 *)
 
 
@@ -101,34 +101,34 @@ lemma "A \<noteq> Server \<Longrightarrow> \<exists>evs \<in> ns_shared.
 
 (*For reasoning about the encrypted portion of message NS3*)
 lemma NS3_msg_in_parts_spies:
-     "Says S A (Crypt KA \<lbrace>N, B, K, X\<rbrace>) \<in> set evs \<Longrightarrow> X \<in> parts (spies evs)"
+     "Says S A (Crypt KA \\<lbrace>N, B, K, X\\<rbrace>) \\<in> set evs \\<Longrightarrow> X \\<in> parts (spies evs)"
 by blast
 
 (*For reasoning about the Oops message*)
 lemma Oops_parts_spies:
-     "Says Server A (Crypt (shrK A) \<lbrace>NA, B, K, X\<rbrace>) \<in> set evs
-            \<Longrightarrow> K \<in> parts (spies evs)"
+     "Says Server A (Crypt (shrK A) \\<lbrace>NA, B, K, X\\<rbrace>) \\<in> set evs
+            \\<Longrightarrow> K \\<in> parts (spies evs)"
 by blast
 
-(** Theorems of the form X \<notin> parts (spies evs) imply that NOBODY
+(** Theorems of the form X \\<notin> parts (spies evs) imply that NOBODY
     sends messages containing X! **)
 
 (*Spy never sees another agent's shared key! (unless it's bad at start)*)
 lemma Spy_see_shrK [simp]:
-     "evs \<in> ns_shared \<Longrightarrow> (Key (shrK A) \<in> parts (spies evs)) = (A \<in> bad)"
+     "evs \\<in> ns_shared \\<Longrightarrow> (Key (shrK A) \\<in> parts (spies evs)) = (A \\<in> bad)"
 apply (erule ns_shared.induct, force, drule_tac [4] NS3_msg_in_parts_spies)
 apply simp_all
 apply blast+;
 done
 
 lemma Spy_analz_shrK [simp]:
-     "evs \<in> ns_shared \<Longrightarrow> (Key (shrK A) \<in> analz (spies evs)) = (A \<in> bad)"
+     "evs \\<in> ns_shared \\<Longrightarrow> (Key (shrK A) \\<in> analz (spies evs)) = (A \\<in> bad)"
 by auto
 
 
 (*Nobody can have used non-existent keys!*)
 lemma new_keys_not_used [rule_format, simp]:
-    "evs \<in> ns_shared \<Longrightarrow> Key K \<notin> used evs \<longrightarrow> K \<notin> keysFor (parts (spies evs))"
+    "evs \\<in> ns_shared \\<Longrightarrow> Key K \\<notin> used evs \\<longrightarrow> K \\<notin> keysFor (parts (spies evs))"
 apply (erule ns_shared.induct, force, drule_tac [4] NS3_msg_in_parts_spies)
 apply simp_all
 (*Fake, NS2, NS4, NS5*)
@@ -140,48 +140,48 @@ done
 
 (*Describes the form of K, X and K' when the Server sends this message.*)
 lemma Says_Server_message_form:
-     "\<lbrakk>Says Server A (Crypt K' \<lbrace>N, Agent B, Key K, X\<rbrace>) \<in> set evs;
-       evs \<in> ns_shared\<rbrakk>
-      \<Longrightarrow> K \<notin> range shrK \<and>
-          X = (Crypt (shrK B) \<lbrace>Key K, Agent A\<rbrace>) \<and>
+     "\\<lbrakk>Says Server A (Crypt K' \\<lbrace>N, Agent B, Key K, X\\<rbrace>) \\<in> set evs;
+       evs \\<in> ns_shared\\<rbrakk>
+      \\<Longrightarrow> K \\<notin> range shrK \\<and>
+          X = (Crypt (shrK B) \\<lbrace>Key K, Agent A\\<rbrace>) \\<and>
           K' = shrK A"
 by (erule rev_mp, erule ns_shared.induct, auto)
 
 
 (*If the encrypted message appears then it originated with the Server*)
 lemma A_trusts_NS2:
-     "\<lbrakk>Crypt (shrK A) \<lbrace>NA, Agent B, Key K, X\<rbrace> \<in> parts (spies evs);
-       A \<notin> bad;  evs \<in> ns_shared\<rbrakk>
-      \<Longrightarrow> Says Server A (Crypt (shrK A) \<lbrace>NA, Agent B, Key K, X\<rbrace>) \<in> set evs"
+     "\\<lbrakk>Crypt (shrK A) \\<lbrace>NA, Agent B, Key K, X\\<rbrace> \\<in> parts (spies evs);
+       A \\<notin> bad;  evs \\<in> ns_shared\\<rbrakk>
+      \\<Longrightarrow> Says Server A (Crypt (shrK A) \\<lbrace>NA, Agent B, Key K, X\\<rbrace>) \\<in> set evs"
 apply (erule rev_mp)
 apply (erule ns_shared.induct, force, drule_tac [4] NS3_msg_in_parts_spies)
 apply auto
 done
 
 lemma cert_A_form:
-     "\<lbrakk>Crypt (shrK A) \<lbrace>NA, Agent B, Key K, X\<rbrace> \<in> parts (spies evs);
-       A \<notin> bad;  evs \<in> ns_shared\<rbrakk>
-      \<Longrightarrow> K \<notin> range shrK \<and>  X = (Crypt (shrK B) \<lbrace>Key K, Agent A\<rbrace>)"
+     "\\<lbrakk>Crypt (shrK A) \\<lbrace>NA, Agent B, Key K, X\\<rbrace> \\<in> parts (spies evs);
+       A \\<notin> bad;  evs \\<in> ns_shared\\<rbrakk>
+      \\<Longrightarrow> K \\<notin> range shrK \\<and>  X = (Crypt (shrK B) \\<lbrace>Key K, Agent A\\<rbrace>)"
 by (blast dest!: A_trusts_NS2 Says_Server_message_form)
 
 (*EITHER describes the form of X when the following message is sent,
   OR     reduces it to the Fake case.
   Use Says_Server_message_form if applicable.*)
 lemma Says_S_message_form:
-     "\<lbrakk>Says S A (Crypt (shrK A) \<lbrace>Nonce NA, Agent B, Key K, X\<rbrace>) \<in> set evs;
-       evs \<in> ns_shared\<rbrakk>
-      \<Longrightarrow> (K \<notin> range shrK \<and> X = (Crypt (shrK B) \<lbrace>Key K, Agent A\<rbrace>))
-          \<or> X \<in> analz (spies evs)"
+     "\\<lbrakk>Says S A (Crypt (shrK A) \\<lbrace>Nonce NA, Agent B, Key K, X\\<rbrace>) \\<in> set evs;
+       evs \\<in> ns_shared\\<rbrakk>
+      \\<Longrightarrow> (K \\<notin> range shrK \\<and> X = (Crypt (shrK B) \\<lbrace>Key K, Agent A\\<rbrace>))
+          \\<or> X \\<in> analz (spies evs)"
 by (blast dest: Says_imp_knows_Spy cert_A_form analz.Inj)
 
 
 (*Alternative version also provable
 lemma Says_S_message_form2:
-  "\<lbrakk>Says S A (Crypt (shrK A) \<lbrace>Nonce NA, Agent B, Key K, X\<rbrace>) \<in> set evs;
-    evs \<in> ns_shared\<rbrakk>
-   \<Longrightarrow> Says Server A (Crypt (shrK A) \<lbrace>Nonce NA, Agent B, Key K, X\<rbrace>) \<in> set evs
-       \<or> X \<in> analz (spies evs)"
-apply (case_tac "A \<in> bad")
+  "\\<lbrakk>Says S A (Crypt (shrK A) \\<lbrace>Nonce NA, Agent B, Key K, X\\<rbrace>) \\<in> set evs;
+    evs \\<in> ns_shared\\<rbrakk>
+   \\<Longrightarrow> Says Server A (Crypt (shrK A) \\<lbrace>Nonce NA, Agent B, Key K, X\\<rbrace>) \\<in> set evs
+       \\<or> X \\<in> analz (spies evs)"
+apply (case_tac "A \\<in> bad")
 apply (force dest!: Says_imp_knows_Spy [THEN analz.Inj]);
 by (blast dest!: A_trusts_NS2 Says_Server_message_form)
 *)
@@ -190,8 +190,8 @@ by (blast dest!: A_trusts_NS2 Says_Server_message_form)
 (****
  SESSION KEY COMPROMISE THEOREM.  To prove theorems of the form
 
-  Key K \<in> analz (insert (Key KAB) (spies evs)) \<Longrightarrow>
-  Key K \<in> analz (spies evs)
+  Key K \\<in> analz (insert (Key KAB) (spies evs)) \\<Longrightarrow>
+  Key K \\<in> analz (spies evs)
 
  A more general formula must be proved inductively.
 ****)
@@ -199,9 +199,9 @@ by (blast dest!: A_trusts_NS2 Says_Server_message_form)
 (*NOT useful in this form, but it says that session keys are not used
   to encrypt messages containing other keys, in the actual protocol.
   We require that agents should behave like this subsequently also.*)
-lemma  "\<lbrakk>evs \<in> ns_shared;  Kab \<notin> range shrK\<rbrakk> \<Longrightarrow>
-         (Crypt KAB X) \<in> parts (spies evs) \<and>
-         Key K \<in> parts {X} \<longrightarrow> Key K \<in> parts (spies evs)"
+lemma  "\\<lbrakk>evs \\<in> ns_shared;  Kab \\<notin> range shrK\\<rbrakk> \\<Longrightarrow>
+         (Crypt KAB X) \\<in> parts (spies evs) \\<and>
+         Key K \\<in> parts {X} \\<longrightarrow> Key K \\<in> parts (spies evs)"
 apply (erule ns_shared.induct, force, drule_tac [4] NS3_msg_in_parts_spies)
 apply simp_all
 (*Fake*)
@@ -216,10 +216,10 @@ done
 (*The equality makes the induction hypothesis easier to apply*)
 
 lemma analz_image_freshK [rule_format]:
- "evs \<in> ns_shared \<Longrightarrow>
-   \<forall>K KK. KK \<subseteq> - (range shrK) \<longrightarrow>
-             (Key K \<in> analz (Key`KK \<union> (spies evs))) =
-             (K \<in> KK \<or> Key K \<in> analz (spies evs))"
+ "evs \\<in> ns_shared \\<Longrightarrow>
+   \\<forall>K KK. KK \\<subseteq> - (range shrK) \\<longrightarrow>
+             (Key K \\<in> analz (Key`KK \\<union> (spies evs))) =
+             (K \\<in> KK \\<or> Key K \\<in> analz (spies evs))"
 apply (erule ns_shared.induct, force)
 apply (drule_tac [7] Says_Server_message_form)
 apply (erule_tac [4] Says_S_message_form [THEN disjE])
@@ -229,9 +229,9 @@ done
 
 
 lemma analz_insert_freshK:
-     "\<lbrakk>evs \<in> ns_shared;  KAB \<notin> range shrK\<rbrakk> \<Longrightarrow>
-       Key K \<in> analz (insert (Key KAB) (spies evs)) =
-       (K = KAB \<or> Key K \<in> analz (spies evs))"
+     "\\<lbrakk>evs \\<in> ns_shared;  KAB \\<notin> range shrK\\<rbrakk> \\<Longrightarrow>
+       Key K \\<in> analz (insert (Key KAB) (spies evs)) =
+       (K = KAB \\<or> Key K \\<in> analz (spies evs))"
 by (simp only: analz_image_freshK analz_image_freshK_simps)
 
 
@@ -239,9 +239,9 @@ by (simp only: analz_image_freshK analz_image_freshK_simps)
 
 (*In messages of this form, the session key uniquely identifies the rest*)
 lemma unique_session_keys:
-     "\<lbrakk>Says Server A (Crypt (shrK A) \<lbrace>NA, Agent B, Key K, X\<rbrace>) \<in> set evs;
-       Says Server A' (Crypt (shrK A') \<lbrace>NA', Agent B', Key K, X'\<rbrace>) \<in> set evs;
-       evs \<in> ns_shared\<rbrakk> \<Longrightarrow> A=A' \<and> NA=NA' \<and> B=B' \<and> X = X'"
+     "\\<lbrakk>Says Server A (Crypt (shrK A) \\<lbrace>NA, Agent B, Key K, X\\<rbrace>) \\<in> set evs;
+       Says Server A' (Crypt (shrK A') \\<lbrace>NA', Agent B', Key K, X'\\<rbrace>) \\<in> set evs;
+       evs \\<in> ns_shared\\<rbrakk> \\<Longrightarrow> A=A' \\<and> NA=NA' \\<and> B=B' \\<and> X = X'"
 apply (erule rev_mp, erule rev_mp, erule ns_shared.induct)
 apply simp_all
 apply blast+
@@ -252,12 +252,12 @@ done
 
 (*Beware of [rule_format] and the universal quantifier!*)
 lemma secrecy_lemma:
-     "\<lbrakk>Says Server A (Crypt (shrK A) \<lbrace>NA, Agent B, Key K,
-                                      Crypt (shrK B) \<lbrace>Key K, Agent A\<rbrace>\<rbrace>)
-              \<in> set evs;
-         A \<notin> bad;  B \<notin> bad;  evs \<in> ns_shared\<rbrakk>
-      \<Longrightarrow> (\<forall>NB. Notes Spy \<lbrace>NA, NB, Key K\<rbrace> \<notin> set evs) \<longrightarrow>
-         Key K \<notin> analz (spies evs)"
+     "\\<lbrakk>Says Server A (Crypt (shrK A) \\<lbrace>NA, Agent B, Key K,
+                                      Crypt (shrK B) \\<lbrace>Key K, Agent A\\<rbrace>\\<rbrace>)
+              \\<in> set evs;
+         A \\<notin> bad;  B \\<notin> bad;  evs \\<in> ns_shared\\<rbrakk>
+      \\<Longrightarrow> (\\<forall>NB. Notes Spy \\<lbrace>NA, NB, Key K\\<rbrace> \\<notin> set evs) \\<longrightarrow>
+         Key K \\<notin> analz (spies evs)"
 apply (erule rev_mp)
 apply (erule ns_shared.induct, force)
 apply (frule_tac [7] Says_Server_message_form)
@@ -277,10 +277,10 @@ done
 
 (*Final version: Server's message in the most abstract form*)
 lemma Spy_not_see_encrypted_key:
-     "\<lbrakk>Says Server A (Crypt K' \<lbrace>NA, Agent B, Key K, X\<rbrace>) \<in> set evs;
-       \<forall>NB. Notes Spy \<lbrace>NA, NB, Key K\<rbrace> \<notin> set evs;
-       A \<notin> bad;  B \<notin> bad;  evs \<in> ns_shared\<rbrakk>
-      \<Longrightarrow> Key K \<notin> analz (spies evs)"
+     "\\<lbrakk>Says Server A (Crypt K' \\<lbrace>NA, Agent B, Key K, X\\<rbrace>) \\<in> set evs;
+       \\<forall>NB. Notes Spy \\<lbrace>NA, NB, Key K\\<rbrace> \\<notin> set evs;
+       A \\<notin> bad;  B \\<notin> bad;  evs \\<in> ns_shared\\<rbrakk>
+      \\<Longrightarrow> Key K \\<notin> analz (spies evs)"
 by (blast dest: Says_Server_message_form secrecy_lemma)
 
 
@@ -288,12 +288,12 @@ by (blast dest: Says_Server_message_form secrecy_lemma)
 
 (*If the encrypted message appears then it originated with the Server*)
 lemma B_trusts_NS3:
-     "\<lbrakk>Crypt (shrK B) \<lbrace>Key K, Agent A\<rbrace> \<in> parts (spies evs);
-       B \<notin> bad;  evs \<in> ns_shared\<rbrakk>
-      \<Longrightarrow> \<exists>NA. Says Server A
-               (Crypt (shrK A) \<lbrace>NA, Agent B, Key K,
-                                 Crypt (shrK B) \<lbrace>Key K, Agent A\<rbrace>\<rbrace>)
-              \<in> set evs"
+     "\\<lbrakk>Crypt (shrK B) \\<lbrace>Key K, Agent A\\<rbrace> \\<in> parts (spies evs);
+       B \\<notin> bad;  evs \\<in> ns_shared\\<rbrakk>
+      \\<Longrightarrow> \\<exists>NA. Says Server A
+               (Crypt (shrK A) \\<lbrace>NA, Agent B, Key K,
+                                 Crypt (shrK B) \\<lbrace>Key K, Agent A\\<rbrace>\\<rbrace>)
+              \\<in> set evs"
 apply (erule rev_mp)
 apply (erule ns_shared.induct, force, drule_tac [4] NS3_msg_in_parts_spies)
 apply auto
@@ -301,16 +301,16 @@ done
 
 
 lemma A_trusts_NS4_lemma [rule_format]:
-   "evs \<in> ns_shared \<Longrightarrow>
-      Key K \<notin> analz (spies evs) \<longrightarrow>
-      Says Server A (Crypt (shrK A) \<lbrace>NA, Agent B, Key K, X\<rbrace>) \<in> set evs \<longrightarrow>
-      Crypt K (Nonce NB) \<in> parts (spies evs) \<longrightarrow>
-      Says B A (Crypt K (Nonce NB)) \<in> set evs"
+   "evs \\<in> ns_shared \\<Longrightarrow>
+      Key K \\<notin> analz (spies evs) \\<longrightarrow>
+      Says Server A (Crypt (shrK A) \\<lbrace>NA, Agent B, Key K, X\\<rbrace>) \\<in> set evs \\<longrightarrow>
+      Crypt K (Nonce NB) \\<in> parts (spies evs) \\<longrightarrow>
+      Says B A (Crypt K (Nonce NB)) \\<in> set evs"
 apply (erule ns_shared.induct, force, drule_tac [4] NS3_msg_in_parts_spies)
 apply (analz_mono_contra, simp_all)
 apply blast     (*Fake*)
 (*NS2: contradiction from the assumptions
-  Key K \<notin> used evs2  and Crypt K (Nonce NB) \<in> parts (spies evs2) *)
+  Key K \\<notin> used evs2  and Crypt K (Nonce NB) \\<in> parts (spies evs2) *)
 apply (force dest!: Crypt_imp_keysFor)
 apply blast     (*NS3*)
 (*NS4*)
@@ -321,11 +321,11 @@ done
 
 (*This version no longer assumes that K is secure*)
 lemma A_trusts_NS4:
-     "\<lbrakk>Crypt K (Nonce NB) \<in> parts (spies evs);
-       Crypt (shrK A) \<lbrace>NA, Agent B, Key K, X\<rbrace> \<in> parts (spies evs);
-       \<forall>NB. Notes Spy \<lbrace>NA, NB, Key K\<rbrace> \<notin> set evs;
-       A \<notin> bad;  B \<notin> bad;  evs \<in> ns_shared\<rbrakk>
-      \<Longrightarrow> Says B A (Crypt K (Nonce NB)) \<in> set evs"
+     "\\<lbrakk>Crypt K (Nonce NB) \\<in> parts (spies evs);
+       Crypt (shrK A) \\<lbrace>NA, Agent B, Key K, X\\<rbrace> \\<in> parts (spies evs);
+       \\<forall>NB. Notes Spy \\<lbrace>NA, NB, Key K\\<rbrace> \\<notin> set evs;
+       A \\<notin> bad;  B \\<notin> bad;  evs \\<in> ns_shared\\<rbrakk>
+      \\<Longrightarrow> Says B A (Crypt K (Nonce NB)) \\<in> set evs"
 by (blast intro: A_trusts_NS4_lemma
           dest: A_trusts_NS2 Spy_not_see_encrypted_key)
 
@@ -333,11 +333,11 @@ by (blast intro: A_trusts_NS4_lemma
   component X in some instance of NS4.  Perhaps an interesting property,
   but not needed (after all) for the proofs below.*)
 theorem NS4_implies_NS3 [rule_format]:
-  "evs \<in> ns_shared \<Longrightarrow>
-     Key K \<notin> analz (spies evs) \<longrightarrow>
-     Says Server A (Crypt (shrK A) \<lbrace>NA, Agent B, Key K, X\<rbrace>) \<in> set evs \<longrightarrow>
-     Crypt K (Nonce NB) \<in> parts (spies evs) \<longrightarrow>
-     (\<exists>A'. Says A' B X \<in> set evs)"
+  "evs \\<in> ns_shared \\<Longrightarrow>
+     Key K \\<notin> analz (spies evs) \\<longrightarrow>
+     Says Server A (Crypt (shrK A) \\<lbrace>NA, Agent B, Key K, X\\<rbrace>) \\<in> set evs \\<longrightarrow>
+     Crypt K (Nonce NB) \\<in> parts (spies evs) \\<longrightarrow>
+     (\\<exists>A'. Says A' B X \\<in> set evs)"
 apply (erule ns_shared.induct, force, drule_tac [4] NS3_msg_in_parts_spies)
 apply analz_mono_contra
 apply (simp_all add: ex_disj_distrib)
@@ -352,13 +352,13 @@ done
 
 
 lemma B_trusts_NS5_lemma [rule_format]:
-  "\<lbrakk>B \<notin> bad;  evs \<in> ns_shared\<rbrakk> \<Longrightarrow>
-     Key K \<notin> analz (spies evs) \<longrightarrow>
+  "\\<lbrakk>B \\<notin> bad;  evs \\<in> ns_shared\\<rbrakk> \\<Longrightarrow>
+     Key K \\<notin> analz (spies evs) \\<longrightarrow>
      Says Server A
-	  (Crypt (shrK A) \<lbrace>NA, Agent B, Key K,
-			    Crypt (shrK B) \<lbrace>Key K, Agent A\<rbrace>\<rbrace>) \<in> set evs \<longrightarrow>
-     Crypt K \<lbrace>Nonce NB, Nonce NB\<rbrace> \<in> parts (spies evs) \<longrightarrow>
-     Says A B (Crypt K \<lbrace>Nonce NB, Nonce NB\<rbrace>) \<in> set evs"
+	  (Crypt (shrK A) \\<lbrace>NA, Agent B, Key K,
+			    Crypt (shrK B) \\<lbrace>Key K, Agent A\\<rbrace>\\<rbrace>) \\<in> set evs \\<longrightarrow>
+     Crypt K \\<lbrace>Nonce NB, Nonce NB\\<rbrace> \\<in> parts (spies evs) \\<longrightarrow>
+     Says A B (Crypt K \\<lbrace>Nonce NB, Nonce NB\\<rbrace>) \\<in> set evs"
 apply (erule ns_shared.induct, force, drule_tac [4] NS3_msg_in_parts_spies)
 apply analz_mono_contra
 apply simp_all
@@ -374,11 +374,11 @@ done
 
 (*Very strong Oops condition reveals protocol's weakness*)
 lemma B_trusts_NS5:
-     "\<lbrakk>Crypt K \<lbrace>Nonce NB, Nonce NB\<rbrace> \<in> parts (spies evs);
-       Crypt (shrK B) \<lbrace>Key K, Agent A\<rbrace> \<in> parts (spies evs);
-       \<forall>NA NB. Notes Spy \<lbrace>NA, NB, Key K\<rbrace> \<notin> set evs;
-       A \<notin> bad;  B \<notin> bad;  evs \<in> ns_shared\<rbrakk>
-      \<Longrightarrow> Says A B (Crypt K \<lbrace>Nonce NB, Nonce NB\<rbrace>) \<in> set evs"
+     "\\<lbrakk>Crypt K \\<lbrace>Nonce NB, Nonce NB\\<rbrace> \\<in> parts (spies evs);
+       Crypt (shrK B) \\<lbrace>Key K, Agent A\\<rbrace> \\<in> parts (spies evs);
+       \\<forall>NA NB. Notes Spy \\<lbrace>NA, NB, Key K\\<rbrace> \\<notin> set evs;
+       A \\<notin> bad;  B \\<notin> bad;  evs \\<in> ns_shared\\<rbrakk>
+      \\<Longrightarrow> Says A B (Crypt K \\<lbrace>Nonce NB, Nonce NB\\<rbrace>) \\<in> set evs"
 by (blast intro: B_trusts_NS5_lemma
           dest: B_trusts_NS3 Spy_not_see_encrypted_key)
 
