src/HOL/Auth/Kerberos_BAN.thy
@@ -30,10 +30,10 @@ consts
 
 rules
     (*The ticket should remain fresh for two journeys on the network at least*)
-    SesKeyLife_LB    "2 <= SesKeyLife"
+    SesKeyLife_LB "#2 <= SesKeyLife"
 
     (*The authenticator only for one journey*)
-    AutLife_LB    "1 <= AutLife"
+    AutLife_LB    "1' <= AutLife"
 
 translations
    "CT" == "length"
